\documentclass{amsart}
\usepackage[ocgcolorlinks,linktoc=all]{hyperref}
\hypersetup{citecolor=blue,linkcolor=red}
\newtheorem{theorem}{Theorem}
\newtheorem*{thmA}{Theorem}
\newtheorem*{thmB}{Theorem}
\newtheorem*{rem}{Remark}
\newtheorem*{thmmain}{Theorem}
\newtheorem{lemma}[theorem]{Lemma}
\newtheorem{proposition}[theorem]{Proposition}
\newtheorem*{propmain}{Proposition}
\newtheorem{corollary}[theorem]{Corollary}
\theoremstyle{definition}
\newtheorem{definition}[theorem]{Definition}
\newtheorem{example}[theorem]{Example}
\newtheorem{xca}[theorem]{Exercise}

\theoremstyle{remark}
\newtheorem{remark}[theorem]{Remark}

\newcommand{\abs}[1]{\lvert#1\rvert}
\numberwithin{equation}{section}

\newcommand{\blankbox}[2]{%
  \parbox{\columnwidth}{\centering
    \setlength{\fboxsep}{0pt}%
    \fbox{\raisebox{0pt}[#2]{\hspace{#1}}}%
  }%
}

\input{StandardPaper2.tex}




\begin{document}

\title[]
 {Harnack estimates for curvature flow equations in space forms}

\curraddr{}
\email{}
\date{\today}

\dedicatory{}
\subjclass[2010]{}
\keywords{}

\begin{abstract}
%We prove differential Harnack inequalities for weakly convex hypersurfaces on the unit sphere shrinking by positive powers of homogeneous degree one, inverse-concave functions of principal curvatures, $f^{\alpha}>0,~\alpha\geq 1$ . As an application, we prove that the only convex, ancient solutions of curvature flows with $f$ concave and inverse-concave velocities are shrinking geodesic spheres.
\end{abstract}

\maketitle

\section{Introduction}

We consider the evolution of a hypersurface $M^n$ by
\[
\partial_tx=-\varphi\nu,~ x:M^n\times[0,T)\to M_K,
\]
where \(M_K\) is the simply connected space form of constant sectional curvature \(K\) and where $\varphi$ is a function on positive, symmetric linear transformations, evaluated at the Weingarten map,
\[
\varphi = \varphi(\mathcal{W}).
\]
Equivalently, \(\varphi\) is a symmetric function on the eigenvalues of \(\mathcal{W}\) (principal curvatures) \(\kappa_1, \cdots, \kappa_n\).

We are particularly interested in the case \(\varphi = f^{\alpha}\) where \(f\) is homogeneous degree one, inverse concave (concave also?) and \(\alpha \in (0,1)\). Our principal result is a Harnack inequality for these flows, extending the inequality in \cite{2015arXiv150802821B, bryanlouie} and inspired by \cite{MR1316556, MR1100812, MR1296393, MR1480081}. Namely, we prove that if \(\varphi = H^{\alpha}\) for \(0 < \alpha \leq 1\) we have

\begin{theorem}
If $\frac{1}{2}+\frac{1}{2n}\leq {\alpha}< 1,$ then
\[
\partial_t H^{\alpha} - b^{ij}\nabla_iH^{\alpha}\nabla_jH^{\alpha} - \frac{K {\alpha}}{2{\alpha}-1}H^{2{\alpha}-1} + \frac{{\alpha}}{{\alpha}+1} \frac{H^{\alpha}}{t} > 0.
\]
If $0<{\alpha}\leq \frac{1}{2} + \frac{1}{2n}$ or ${\alpha}=1$, then
\[
\partial_t H^{\alpha} - b^{ij}\nabla_iH^{\alpha}\nabla_jH^{\alpha} - K n{\alpha}H^{2{\alpha}-1} + \frac{{\alpha}}{{\alpha}+1} \frac{H^{\alpha}}{t} > 0.
\]
\end{theorem}

\section{Preliminaries}

Let $\overline{g}$ and $\overline{Rm}$ denote, respectively, the metric and the curvature tensor of $M_K$. Define \(M_t := x(M^n,t)\), and let \(g = x_t^{\ast} \overline{g}\) denote the induced metric on \(M\) with $\nabla$ the corresponding Levi-Civita connection. Write $\nu$ for the outer unit normal to $M_t$ and let \(\{\partial_i\}_{i=1}^n\) be a local frame on \(M\) which extends to a frame \(\{\partial_0 = \nu, (x_t)_{\ast} \partial_1, \cdots, (x_t)_{\ast} \partial_n\}\) on \(M_K\) in a neighbourhood of \(M_t\). 

Let Greek indices range from \(0\) to \(n\) and Latin indices range from \(1\) to \(n\). The Riemann curvature tensor of \(M_K\) satisfies \(\bar{R}_{\alpha\beta\gamma\theta} = K(\bar{g}_{\alpha\gamma}\bar{g}_{\beta\delta} - \bar{g}_{\alpha\theta}\bar{g}_{\beta\gamma})\). We may write the metric $g = \{g_{ij}\}$, second fundamental form $A = \{h_{ij}\}$, the Weingarten map $\mathcal{W} = h^i_j = g^{mi} h_{jm}$ and the Riemann curvature tensor $Rm_{ijkl}$ with respect to the given frame. We shall write \(\nabla_i\) for covariant derivatives and also use the notation \(\nabla^i = g^{ik} \nabla_k\). Second covariant derivatives will be written \(\nabla^2_{ij}\) and \((\nabla^2)^i_j\). The mean curvature of $M^n$ is the trace of the Weingarten map (equivalently the trace of the second fundamental form with respect to $g$), $H = g^{ij}h_{ij} = h^i_i$.

We use the following standard notation
\[
(h^2)_i^j = g^{mj}g^{rs}h_{ir}h_{sm},
\]
\[
(h^2)_{ij} = g_{kj} (h^2)_i^k = h^k_i h_{kj},
\]
\[
|A|^2 = g^{ij}g^{kl}h_{ik}h_{lj} = h_{ij}h^{ij},
\]
Here, $\{g^{ij}\}$ is the inverse matrix of $\{g_{ij}\}.$ For a strictly convex hypersurface, \(A\) is strictly positive-definite and hence has a strictly positive-definite inverse, which we denote by \(b = \{b^{ij}\}\).

The relations between $A$, $Rm$, and $\overline{Rm}$ are given by the Gau{\ss} and Codazzi equations:
\[
\begin{split}
Rm_{ijkl} &= \overline{Rm}_{ijkl} + h_{ik}h_{jl} - h_{il}h_{jk} \\
&= K(\bar{g}_{ik}\bar{g}_{jl} - \bar{g}_{il}\bar{g}_{jk}) + h_{ik}h_{jl} - h_{il}h_{jk},
\end{split}
\]
\[
\nabla_i h_{jk} = \nabla_k h_{ij},
\]
valid for space forms. We also make use of the Ricci identity,
\[
{R_{ijk}}^m  = \left(\nabla^2_{i, j} \partial_k - \nabla^2_{j,i} \partial_k\right)^m
\]

We also need some notation for derivatives of the speed \(\phi\). Let us write
\[
\varphi^{i}_{j} = \frac{\partial \varphi}{\partial h^{j}_{i}}
\]
for the first partial derivatives of \(\varphi\). We may also think of \(\varphi\) as a function of the metric and second fundamental form
\[
\varphi(g, h) = \varphi(g^{ik} h_{kj}).
\]
From this point of view, for the first and second partial derivatives, let us write
\[
\varphi^{ij} = \frac{\partial\varphi}{\partial h_{ij}}, \quad \varphi^{ij,kl} = \fr{\partial^2\varphi}{\partial h_{kl} \partial h_{ij}}.
\]
and define the operator
\[
\Box = \varphi^{ij} \nabla^2_{ij}.
\]

We frequently make use, without comment, of the formula for differentiating an inverse
\[
\frac{\partial g^{ij}}{\partial g_{kl}} = - g^{kj} g^{il}.
\]

First derivatives of \(\phi\) from the two perspectives are related by
\begin{equation}
\label{eq:delh}
\varphi^{ij} = \frac{\partial \phi}{\partial h_l^k} \frac{\partial h_l^k}{\partial h_{ij}} = \varphi^l_k g^{ik} \delta^j_l = g^{ik} \varphi^j_k.
\end{equation}
and
\begin{equation}
\label{eq:delg}
\frac{\partial\varphi}{\partial g_{ij}} = \varphi^{l}_{k} \frac{\partial h^{k}_{l}}{\partial g_{ij}} = -\varphi^{l}_{k} g^{ki} g^{rj} h_{rl} = -\varphi^{li}h^{j}_{l}.
\end{equation}
We will also need the mixed second derivatives,
\begin{equation}
\label{eq:delhdelg}
\begin{split}
\frac{\partial \varphi^{ij}}{\partial g_{kl}} &= \frac{\partial}{\partial g_{kl}} \left(g^{sj} \varphi^{i}_{s} \right) = - g^{kj}g^{sl} \varphi^{i}_{s} - g^{sj} (\phi^i_s)^{mk} h^l_m \\
&= - g^{kj} \varphi^{il} - g^{sj} g_{ns} \phi^{in,mk} h^l_m \\
&= - g^{kj} \varphi^{il} - \phi^{ij,mk} h^l_m
\end{split}
\end{equation}
where we applied equation \eqref{eq:delg} to \(\phi^i_s\) in the first line.

\section{Evolution equations}

The evolution equations in the following lemma are standard and can be found in many places \cite{MR1316556, MR1100812, MR1296393, MR1480081}. The basic tools are commuting derivatives, using the definition of the curvature tensor for space forms, the Gauss equation, and the Codazzi equation as described in the previous section. Compare also \cite[p.~94-95]{Gerhardt:/2006} and the formula \cite[eq.~(6.17)]{Gerhardt:01/1996}.

\begin{lemma}
\label{lem:evolution}
The following evolution equations hold
\begin{enumerate}
  \item \label{eq:delt_metric} $\partial_tg_{ij} = -2\varphi h_{ij}$
  \item \label{eq:delt_inversemetric} $\partial_t g^{ij} = 2\varphi h^{ij}$
  \item \label{eq:delt_christoffel} $\partial_t {\G}^{k}_{ij} = -\varphi g^{kl} \nabla_l h_{ij} - h^k_i \nabla_j \varphi - h^k_j \nabla_i \varphi + g^{kl} h_{ij} \nabla_l \varphi$
  \item \label{eq:delt_sff} $\partial_t h_{ij} = \nabla^2_{ji} \varphi - \varphi(h^2)_{ij} + K \varphi g_{ij}$
  \item \label{eq:delt_weingarten} $\partial_t h_i^j = (\nabla^2)^j_i\varphi + \varphi(h^2)_i^j + K \varphi\delta_i^j$
  \item \label{eq:delt_sff_box} \begin{align*}
\partial_t h_{ij} &= \Box h_{ij} + \varphi^{kl} (h^2)_{kl} h_{ij} - (\varphi'f + \varphi) (h^2)_{ij} \\
& \quad + \varphi^{kl,rs}\nabla_i h_{kl}\nabla_j h_{rs} \\
& \quad + K \{(\varphi + \varphi'f) g_{ij} - \varphi^{kl}g_{kl}h_{ij}\}
\end{align*}
  \item \label{eq:delt_weingarten_box} \begin{align*}
\partial_t h_i^j &= \Box h_i^j + \varphi^{kl} (h^2)_{kl} h_i^j - (\varphi'f - \varphi) (h^2)_i^j \\
& \quad + \varphi^{kl,rs}\nabla_i h_{kl}\nabla^j h_{rs} \\
& \quad + K \{(\varphi + \varphi'f) \delta_i^j - \varphi^{kl}g_{kl}h_i^j\}
\end{align*}
  \item \label{eq:delt_inversesff} \begin{align*}
\partial_t b^{ij} &= \Box b^{ij} - \varphi^{rs} (h^2)_{rs} b^{ij} + (\varphi'f + \varphi) g^{ij} \\  
& \quad - \left(2b^{lq}\varphi^{kp} + \varphi^{kl,pq}\right) b^{ir}b^{js} \nabla_r h_{kl} \nabla_s h_{pq} \\
& \quad - K \{(\varphi + \varphi'f) b^{ir}b^{j}_{r} + \varphi^{kl}g_{kl}b^{ij}\}
\end{align*}
  \item \label{eq:delt_speed} $\partial_t \varphi = \Box \varphi + \varphi\varphi^{ij}(h^2)_{ij} + K \varphi\varphi^{ij}g_{ij}$
\end{enumerate}
\end{lemma}

\begin{lemma}
\label{lem:deltBox}
The following commutation relation holds
\[
\begin{split}
(\partial_{t}\Box - \Box\partial_{t}) \varphi &= \varphi^{ij,kl} \nabla^2_{i,j} \varphi (\nabla^2_{k,l} \varphi + \varphi (h^2)_{kl} + K \varphi g_{kl}) \\
&\quad + 2\varphi^{ij}h^{k}_{i} (\varphi \nabla^2_{k,j} \varphi + \nabla_k \varphi \nabla_j \varphi) + (\varphi - \varphi^{ij}h_{ij})| \nabla\varphi|^{2}.
\end{split}
\]
\end{lemma}

\begin{proof}
First, let us calculate the evolution of \(\varphi^{ij}\), which will also prove useful later. From the mixed derivative equation \eqref{eq:delhdelg}, the evolution of the metric (Lemma \ref{lem:evolution}, \eqref{eq:delt_metric}), and the evolution of the second fundamental form (Lemma \ref{lem:evolution}, \eqref{eq:delt_sff}) we compute
\begin{equation}
\label{eq:deltBox}
\begin{split}
\partial_{t} \varphi^{ij} &= \varphi^{ij,kl} \partial_t h_{kl} + \frac{\partial\varphi^{ij}}{\partial g_{kl}} \partial_t g_{kl} \\
&= \varphi^{ij,kl} \left(\nabla^2_{k,l} \varphi - \varphi(h^2)_{kl} + K \varphi g_{kl}\right) + 2\varphi \varphi^{ij,kl} h_{lm}h^{m}_{k} + 2\varphi\varphi^{jk}g^{li}h_{kl} \\
&=\varphi^{ij,kl} \left(\nabla^2_{k,l} \varphi + \varphi(h^2)_{kl} + K \varphi g_{kl}\right) + 2\varphi\varphi^{jk}h^{i}_{k}.
\end{split}
\end{equation}

We obtain from equation \eqref{eq:deltBox} and the evolution of the Christoffel symbols (Lemma \ref{lem:evolution}, \eqref{eq:delt_christoffel}),
\[
\begin{split}
\left(\partial_{t}\Box - \Box\partial_{t}\right) \varphi &= \left(\partial_{t}\varphi^{ij}\right) \nabla^2_{i,j} \varphi + \varphi^{ij} \left(\partial_{t} \nabla^2_{i,j} \varphi - \nabla^2_{i,j} \partial_t \varphi\right) \\
&= \left(\partial_{t}\varphi^{ij}\right) \nabla^2_{i,j} \varphi - \varphi^{ij}\partial_t \G^{k}_{ij} \nabla_k \varphi \\
&= \left(\varphi^{ij,kl} \left(\nabla^2_{k,l} \varphi + \varphi(h^2)_{kl} + K \varphi g_{kl}\right) + 2\varphi\varphi^{jk}h^{i}_{k}\right) \nabla^2_{i,j} \varphi \\
&\quad + \varphi^{ij} \nabla_k \varphi \left(\varphi g^{kl} \nabla_l h_{ij} + h^k_i \nabla_j \varphi + h^k_j \nabla_i \varphi - g^{kl} h_{ij} \nabla_l \varphi\right)
\end{split}
\]
The result now follows after rearranging and using \(|\nabla \varphi|^2 = g^{kl}\nabla_k \varphi \nabla_l \varphi\) and \(\nabla_l \varphi = \varphi^{ij} \nabla_l h_{ij}\) by the chain rule.
\end{proof}

\begin{lemma}
\label{lem:gradBox}
For every smooth function $f$, the commutation relation
\[
\begin{split}
(\nabla_i \Box -\Box \nabla_i) f &= \varphi^{kl,rs} \nabla_i h_{rs} \nabla^2_{k,l} f \\
&\quad + K \varphi^{kl} \left(g_{ki} \nabla_l f - g_{kl} \nabla_i f\right) \\
&\quad + \varphi^{kl}\left(h^{m}_{l}h_{ki} - h_{kl}h^{m}_{i}\right) \nabla_m f
\end{split}
\]
holds.
\end{lemma}

\begin{proof}
From the Ricci identities we obtain
\[
\begin{split}
\nabla_i (\varphi^{kl} \nabla^2_{k,l} f) - \varphi^{kl}(\nabla^2_{k,l} \nabla_i f) &= \varphi^{kl,rs} \nabla_i h_{rs} \nabla^2_{k,l}f + \varphi^{kl}(\nabla_i \nabla^2_{k,l} f - \nabla^2_{k,l} \nabla_i f)  \\
&= \varphi^{kl,rs} \nabla_i h_{rs} \nabla^2_{k,l}f \\
& \quad + \varphi^{kl}(\nabla_i \nabla_k \nabla_l f - \nabla_i \nabla_{\nabla_k \partial_l} f - \nabla_k \nabla_l \nabla_i f + \nabla_{\nabla_k \partial_l} \nabla_i f) \\
&= \varphi^{kl,rs} \nabla_i h_{rs} \nabla^2_{k,l}f \\
&\quad + \varphi^{kl}(\nabla_i \nabla_k \nabla_l f - \nabla_k \nabla_i \nabla_l f - \nabla_i \nabla_{\nabla_k \partial_l} f  + \nabla_{\nabla_k \partial_l} \nabla_i f) \\
&= \varphi^{kl,rs} \nabla_i h_{rs} \nabla^2_{k,l}f + \varphi^{kl}{R^{m}}_{kli} \nabla_m f
\end{split}
\]
and from the Gauss equation we obtain
\[
\begin{split}
{R^{m}}_{kli} \nabla_m f &= \left(K\left(g^{pm}g_{ki}g_{pl}  - g^{pm}g_{pi}g_{kl}\right) + g^{pm} h{pl}h_{ki} - g^{pm}h_{kl}h_{pi}\right) \nabla_m f \\
&= K\left(g_{ki} \nabla_l f - g_{kl} \nabla_i f\right) + \left(h^{m}_{l}h_{ki} - h_{kl}h^{m}_{i}\right) \nabla_m f.
\end{split}
\]
\end{proof}


\Theo{lemma}{Evbeta}{
The quantity 
\eq{\b=\dot{\p}-\l\p^{ij}g_{ij}\p=\Box\p+\p^{ij}h_{ik}h^{k}_{j}\p.}
satisfies
\eq{\br{\del_{t}-\Box}\b&=\p^{ij}h_{ik}h^{k}_{j}\b+2\p^{ij}h^{k}_{i}\br{2\p_{;kj}\p+\p_{;k}\p_{;j}+h^{s}_{j}h_{sk}\p^{2}}\\
				&\hp{=}+\br{\p-\p^{ij}h_{ij}}|\nabla\p|^{2}\\
				&\hp{=}+\p^{ij,kl}\br{\p_{;ij}+h_{ip}h^{p}_{j}\p}\br{\p_{;kl}+h^{m}_{k}h_{ml}\p}\\
				&\hp{=}+\l\p^{ij}g_{ij}\b+2\l\p^{rs}\br{\p^{ij}g_{ij}}_{;r}\p_{;s}+\l\Box\br{\p^{ij}g_{ij}}\p\\
				&\hp{=}+\l\p^{ij,rs}g_{rs}\br{\p_{;ij}\p+h_{ik}h^{k}_{j}\p^{2}}+2\l\p^{ij}h_{ij}\p^{2}.}
}

\pf{We will need the following auxillary calculation, where we use \cref{eq:deltBox}.
\eq{\del_{t}\br{\p^{ij}h_{ik}h^{k}_{j}}&=\del_{t}\p^{ij}h_{ik}h^{k}_{j}+\p^{ij}\dot{h}_{ik}h^{k}_{j}+\p^{ij}h_{ik}\dot{h}^{k}_{j}\\
				&=\p^{ij,kl}\br{\dot{h}_{kl}+2\p h_{kr}h^{r}_{l}}h_{ir}h^{r}_{j}+2\p\p^{jk}h^{i}_{k}h_{ir}h^{r}_{j}\\
				&\hp{=}+\p^{ij}\br{\p_{;ik}-\p h^{r}_{i}h_{rk}+\l\p g_{ik}}h^{k}_{j}\\
				&\hp{=}+\p^{ij}\br{{\p_{;j}}^{k}+\p h^{k}_{r}h^{r}_{j}+\l\p\d^{k}_{j}}h_{ik}\\
				&=\p^{ij,kl}\br{\p_{;kl}+\p h^{r}_{k}h_{rl}+\l\p g_{kl}}h_{is}h^{s}_{j}+2\p\p^{jk}h^{i}_{k}h_{ir}h^{r}_{j}\\
				&\hp{=}+2\p^{ij}h^{k}_{i}\p_{;jk}+2\l\p^{ij}h_{ij}\p.}

 We use \cref{lem:deltBox} to compute
\eq{\br{\del_{t}-\Box}\b&=\del_{t}\Box\p+\del_{t}\br{\p^{ij}h_{ik}h^{k}_{j}\p}-\Box\Box\p-\Box\br{\p^{ij}h_{ik}h^{k}_{j}\p}\\
			&=\Box\br{\l\p^{ij}g_{ij}\p}+2\p^{ij}h^{k}_{i}\br{\p_{;kj}\p+\p_{;k}\p_{;j}}+\br{\p-\p^{ij}h_{ij}}|\nabla\p|^{2}\\
					&\hp{=}+\p^{ij,rs}\p_{;ij}\br{\p_{;rs}+\p h_{rm}h^{m}_{s}+\l\p g_{rs}}+\del_{t}\br{\p^{ij}h_{ik}h^{k}_{j}\p}\\
			&=\l\p^{ij}g_{ij}\b-\l\p^{kl}g_{kl}\p^{ij}h_{ir}h^{r}_{j}\p+2\l\p^{rs}\br{\p^{ij}g_{ij}}_{;r}\p_{;s}\\
			&\hp{=}+\l\Box\br{\p^{ij}g_{ij}}\p+2\p^{ij}h^{k}_{i}\br{\p_{;kj}\p+\p_{;k}\p_{;j}}\\
			&\hp{=}+\br{\p-\p^{ij}h_{ij}}|\nabla\p|^{2}+\p^{ij,rs}\p_{;ij}\br{\p_{;rs}+\p h_{rm}h^{m}_{s}+\l\p g_{rs}}\\
			&\hp{=}+\p^{ij}h_{ik}h^{k}_{j}\b+\l\p^{ij}h_{ik}h^{k}_{j}\p^{rs}g_{rs}\p+\del_{t}\br{\p^{ij}h_{ik}h^{k}_{j}}\p\\
			&=\p^{ij}h_{ik}h^{k}_{j}\b+\l\p^{ij}g_{ij}\b+2\l\p^{rs}\br{\p^{ij}g_{ij}}_{;r}\p_{;s}\\
			&\hp{=}+\l\Box\br{\p^{ij}g_{ij}}\p+2\p^{ij}h^{k}_{i}\br{\p_{;kj}\p+\p_{;k}\p_{;j}}	\\
			&\hp{=}+\br{\p-\p^{ij}h_{ij}}|\nabla\p|^{2}+\p^{ij,rs}\p_{;ij}\br{\p_{;rs}+\p h_{rm}h^{m}_{s}+\l\p g_{rs}}\\
			&\hp{=}+\p^{ij,kl}\br{\p_{;kl}+\p h^{r}_{k}h_{rl}+\l\p g_{kl}}h_{is}h^{s}_{j}\p+2\p^{jk}h^{i}_{k}h_{ir}h^{r}_{j}\p^{2}\\
				&\hp{=}+2\p^{ij}h^{k}_{i}\p_{;jk}\p+2\l\p^{ij}h_{ij}\p^{2}.}
}

\Theo{lemma}{Evgradphi}{
There holds
\eq{\br{\del_{t}-\Box}\p_{;i}&=\br{\p^{kl}h_{kr}h^{r}_{l}\p}_{;i}+\l\p^{kl}\p_{;l}g_{ki}+\l\p^{kl,rs}h_{rs;i}g_{kl}\p\\
				&\hp{=}+\p^{kl,rs}h_{rs;i}\p_{;kl}+\br{\p^{kl}h^{m}_{l}h_{ki}-\p^{kl}h_{kl}h^{m}_{i}}\p_{;m}.}
}

\pf{
\eq{\del_{t}\p_{;i}-\Box\p_{;i}&=\br{\Box\p}_{;i}+\br{\p^{kl}h_{rk}h^{r}_{l}\p}_{;i}+\l\br{\p^{kl}g_{kl}\p}_{;i}\\
					&\hp{=}-\br{\Box\p}_{;i}+\p^{kl,rs}h_{rs;i}\p_{;kl}+\l\p^{kl}g_{ki}\p_{;l}-\l\p^{kl}g_{kl}\p_{;i}\\
					&\hp{=}+\p^{kl}h^{m}_{l}h_{ki}\p_{;m}-\p^{kl}h_{kl}h^{m}_{i}\p_{;m}\\
					&=\br{\p^{kl}h_{rk}h^{r}_{l}\p}_{;i}+\l\p^{kl,rs}h_{rs;i}g_{kl}\p+\p^{kl,rs}h_{rs;i}\p_{;kl}\\
					&\hp{=}+\l\p^{kl}g_{ki}\p_{;l}+\br{\p^{kl}h^{m}_{l}h_{ki}-\p^{kl}h_{kl}h^{m}_{i}}\p_{;m}.}
}

\Theo{lemma}{Evtheta}{
The quantity $\t=b^{ij}\p_{;i}\p_{;j}$ satisfies
\eq{\br{\del_{t}-\Box}\t&=\p^{rs}h_{rk}h^{k}_{s}\t-\br{2b^{lq}\p^{kp}+\p^{kl,pq}}b^{ir}b^{js}\p_{;i}\p_{j}h_{kl;r}h_{pq;s}\\
							&\hp{=}+\br{\p'f+\p-2\p^{kl}h_{kl}}|\nabla\p|^{2}+2\p^{jl}h^{m}_{l}\p_{;m}\p_{;j}\\
							&\hp{=}+2b^{ij}\p^{kl,rs}h_{rs;i}\p_{;j}\br{\p_{;kl}+h_{rk}h^{r}_{l}\p}+4b^{ij}\p^{kl}h_{rk;i}h^{r}_{l}\p_{;j}\p\\
							&\hp{=}+4\p^{rs}b^{ip}b^{jq}h_{pq;r}\p_{;is}\p_{;j}-2b^{ij}\p^{rs}\p_{;ir}\p_{;js}\\
							&\hp{=}-\l\br{\p'f+\p}b^{ir}b^{j}_{r}\p_{;i}\p_{;j}+\l\p^{kl}g_{kl}\t+2\l b^{j}_{k}\p^{kl}\p_{;l}\p_{;j}\\
							&\hp{=}+2\l b^{ij}\p^{kl,rs}h_{rs;i}\p_{;j}g_{kl}\p.}
}

\pf{
\eq{\br{\del_{t}-\Box}\t&=\br{\dot{b}^{ij}-\Box b^{ij}}\p_{;i}\p_{;j}+2b^{ij}\br{\dot{\p}_{;i}-\Box\p_{;i}}\p_{;j}\\
							&\hp{=}-4\p^{rs}{b^{ij}}_{;r}\p_{;is}\p_{;j}-2b^{ij}\p^{rs}\p_{;ir}\p_{;js}\\
							&=-\p^{rs}h_{rk}h^{k}_{s}\t+\br{\p'f+\p}|\nabla\p|^{2}-\l\br{\p'f+\p}b^{ir}b^{j}_{r}\p_{;i}\p_{;j}\\
							&\hp{=}+\l\p^{kl}g_{kl}\t-\br{2b^{lq}\p^{kp}+\p^{kl,pq}}b^{ir}b^{js}\p_{;i}\p_{;j}h_{kl;r}h_{pq;s}\\
							&\hp{=}+2\p^{kl}h_{rk}h^{r}_{l}\t+2b^{ij}\br{\p^{kl}h_{rk}h^{r}_{l}}_{;i}\p_{;j}\p+2b^{ij}\p^{kl,rs}h_{rs;i}\p_{;j}\p_{;kl}\\
							&\hp{=}+2b^{ij}\br{\p^{kl}h^{m}_{l}h_{ki}-\p^{kl}h_{kl}h^{m}_{i}}\p_{;m}\p_{;j}\\
							&\hp{=}+2\l b^{ij}\p^{kl,rs}h_{rs;i}\p_{;j}g_{kl}\p+2\l b^{j}_{k}\p^{kl}\p_{;l}\p_{;j}\\
							&\hp{=}-4\p^{rs}{b^{ij}}_{;r}\p_{;is}\p_{;j}-2b^{ij}\p^{rs}\p_{;ir}\p_{;js}\\
							&=\p^{rs}h_{rk}h^{k}_{s}\t-\br{2b^{lq}\p^{kp}+\p^{kl,pq}}b^{ir}b^{js}\p_{;i}\p_{;j}h_{kl;r}h_{pq;s}\\
							&\hp{=}+\br{\p'f+\p}|\nabla\p|^{2}+2\p^{jl}h^{m}_{l}\p_{;m}\p_{;j}-2\p^{kl}h_{kl}|\nabla\p|^{2}\\
							&\hp{=}+2b^{ij}\p^{kl,rs}h_{rs;i}\p_{;j}\br{\p_{;kl}+h_{rk}h^{r}_{l}\p}+4b^{ij}\p^{kl}h_{rk;i}h^{r}_{l}\p_{;j}\p\\
							&\hp{=}-4\p^{rs}{b^{ij}}_{;r}\p_{;is}\p_{;j}-2b^{ij}\p^{rs}\p_{;ir}\p_{;js}\\
							&\hp{=}-\l\br{\p'f+\p}b^{ir}b^{j}_{r}\p_{;i}\p_{;j}+\l\p^{kl}g_{kl}\t+2\l b^{j}_{k}\p^{kl}\p_{;l}\p_{;j}\\
							&\hp{=}+2\l b^{ij}\p^{kl,rs}h_{rs;i}\p_{;j}g_{kl}\p.}
}

\Theo{lemma}{Evchi}{
Let $\d\neq 0.$ The quantity 
\eq{\chi=t(\b-\t)+\d\p}
satisfies
\eq{\dot{\chi}-\Box\chi&=\br{\fr{\b-\t}{\d\p}+\p^{ij}h_{ik}h^{k}_{j}+\l\p^{ij}g_{ij}}\chi\\
				&\hp{=}+t\br{\p^{ij,kl}+2b^{il}\p^{jk}-\fr{\p^{ij}\p^{kl}}{\d\p}}\eta_{ij}\eta_{kl}+t\l R,}
where
\eq{\eta_{ij}=\p_{;ij}-b^{rs}h_{ij;r}\p_{;s}+h_{ip}h^{p}_{j}\p}
and 
\eq{R&=2\p^{rs}\br{\p^{ij}g_{ij}}_{;r}\p_{;s}+\Box\br{\p^{ij}g_{ij}}\p\\
				&\hp{=}+\p^{kl,rs}g_{rs}\br{\p_{;kl}\p+h_{kr}h^{r}_{l}\p^{2}-2b^{ij}h_{kl;i}\p_{;j}\p}+2\p^{ij}h_{ij}\p^{2}\\
				&\hp{=}+\br{\p'f+\p}b^{ir}b^{j}_{r}\p_{;i}\p_{;j}-2 b^{j}_{k}\p^{kl}\p_{;l}\p_{;j}.
}
}
	
\pf{
\eq{\dot\chi&-\Box\chi=\b-\t+t\br{\br{\del_{t}-\Box}\br{\b-\t}}+\d\br{\dot\p-\Box\p}\\
				&=\b-\t+\d\p^{ij}h_{ik}h^{k}_{j}\p+\d\l\p^{ij}g_{ij}\p\\
				&\hp{=}+t\Big(\p^{ij}h_{ik}h^{k}_{j}\br{\b-\t}+\br{\p^{ij}h_{ij}-\p'f}|\nabla\p|^{2}\\
				&\hp{=}+\p^{ij,kl}\br{\p_{;ij}+h_{ip}h^{p}_{j}\p}\br{\p_{;kl}+h^{m}_{k}h_{ml}\p}\\
				&\hp{=}+\p^{ij,kl}b^{pr}b^{sq}\p_{;p}\p_{;q}h_{ij;r}h_{kl;s}-2\p^{ij,kl}b^{rs}h_{kl;r}\p_{;s}\br{\p_{;ij}+h_{ip}h^{p}_{j}\p}\\
				&\hp{=}+2\p^{ik}h^{r}_{i}\br{2\p_{;rk}\p+h^{s}_{k}h_{sr}\p^{2}}+2b^{il}\p^{jk}b^{pr}b^{qs}\p_{;p}\p_{;q}h_{kl;r}h_{ij;s}\\
				&\hp{=}-4b^{il}\p^{jk}h_{rk;i}h^{r}_{j}\p_{;l}\p-4\p^{jk}b^{il}b^{pq}h_{lj;q}\p_{;ik}\p_{;p}+2b^{il}\p^{jk}\p_{;ij}\p_{;lk}\\
				&\hp{=}+\l\p^{ij}g_{ij}\br{\b-\t}+2\l\p^{rs}\br{\p^{ij}g_{ij}}_{;r}\p_{;s}+\l\Box\br{\p^{ij}g_{ij}}\p\\
				&\hp{=}+\l\p^{kl,rs}g_{rs}\br{\p_{;kl}\p+h_{kr}h^{r}_{l}\p^{2}-2b^{ij}h_{kl;i}\p_{;j}\p}+2\l\p^{ij}h_{ij}\p^{2}\\
				&\hp{=}+\l\br{\p'f+\p}b^{ir}b^{j}_{r}\p_{;i}\p_{;j}-2\l b^{j}_{k}\p^{kl}\p_{;l}\p_{;j}\Big)\\
				&=\b-\t+\br{\p^{ij}h_{ik}h^{k}_{j}+\l\p^{ij}g_{ij}}\chi+t\br{\p^{ij}h_{ij}-\p'f}|\nabla\p|^{2}\\
				&\hp{=}+t\p^{ij,kl}\br{\p_{;ij}-b^{rs}h_{ij;r}\p_{;s}+h_{ip}h^{p}_{j}\p}\br{\p_{;kl}-b^{mn}h_{kl;m}\p_{;n}+h_{kq}h^{q}_{l}\p}\\
				&\hp{=}+2tb^{il}\p^{jk}\br{\p_{;ij}-b^{rs}h_{ij;r}\p_{;s}+h_{ip}h^{p}_{j}\p}\br{\p_{;kl}-b^{mn}h_{kl;m}\p_{;n}+h_{kq}h^{q}_{l}\p}\\
				&\hp{=}+2t\l\p^{rs}\br{\p^{ij}g_{ij}}_{;r}\p_{;s}+t\l\Box\br{\p^{ij}g_{ij}}\p\\
				&\hp{=}+t\l\p^{kl,rs}g_{rs}\br{\p_{;kl}\p+h_{kr}h^{r}_{l}\p^{2}-2b^{ij}h_{kl;i}\p_{;j}\p}+2t\l\p^{ij}h_{ij}\p^{2}\\
				&\hp{=}+t\l\br{\p'f+\p}b^{ir}b^{j}_{r}\p_{;i}\p_{;j}-2t\l b^{j}_{k}\p^{kl}\p_{;l}\p_{;j}.
}
}			
	


\bibliographystyle{amsplain}
\bibliography{Bibliography.bib}


\end{document}
